wip on ordered: towards an append lemma.

src/spec/Flutterbye.Seq.Ordered.fst
@@ -35,8 +35,25 @@ private type transitive_p (#a_t:Type) (f:cmp_t a_t) (s:seq a_t) =
    forall x y z.
       mem_p x s /\ mem_p y s /\ mem_p z s /\ b2t (f x y && f y z) ==> f x z
 
+private type sequenced_p (#a_t:Type) (f:cmp_t a_t) (s:seq a_t) =
+   length s < 2
+   \/ (forall (x:nat) (y:nat).
+         (x < length s && y < length s && x < y)
+         ==> (
+            x < length s && y < length s
+            && (
+               let a_x = index s x in
+               let a_y = index s y in
+               not (f a_y a_x) && (f a_x a_y)
+            )
+         )
+      )
+
 type pordered_p (#a_t:Type) (f:cmp_t a_t) (s:seq a_t) =
-   reflexive_p f s /\ antisymmetric_p f s /\ transitive_p f s
+   reflexive_p f s
+   /\ antisymmetric_p f s
+   /\ transitive_p f s
+   /\ sequenced_p f s
 
 private val reflexive_loop:
    f:cmp_t 'a ->
@@ -45,7 +62,7 @@ private val reflexive_loop:
    Tot (b:bool{b2t b <==> reflexive_p f s})
       (decreases (length s - i))
 let rec reflexive_loop f s i =
-   slice_lemma s;
+   Flutterbye.Seq.Mem.slice_lemma s;
    if i < length s then
       let a = index s i in
       if f a a then
@@ -67,7 +84,7 @@ private val antisymmetric_inner_loop:
    Tot (b:bool{b2t b <==> antisymmetric_inner_p f s a})
       (decreases (length s - i))
 let rec antisymmetric_inner_loop f s a i =
-   slice_lemma s;
+   Flutterbye.Seq.Mem.slice_lemma s;
    if i < length s then
       let a' = index s i in
       if (a = a') = (f a a' && f a' a) then
@@ -84,7 +101,7 @@ private val antisymmetric_loop:
    Tot (b:bool{b2t b <==> antisymmetric_p f s})
       (decreases (length s - i))
 let rec antisymmetric_loop f s i =
-   slice_lemma s;
+   Flutterbye.Seq.Mem.slice_lemma s;
    if i < length s then
       let a = index s i in
       if antisymmetric_inner_loop f s a 0 then
@@ -107,7 +124,7 @@ private val transitive_loop_z:
    Tot (b:bool{b2t b <==> transitive_loop_z_p f s a_1 a_2})
       (decreases (length s - i))
 let rec transitive_loop_z f s a_1 a_2 i =
-   slice_lemma s;
+   Flutterbye.Seq.Mem.slice_lemma s;
    if i < length s then
       let a_3 = index s i in
       if f a_1 a_2 && f a_2 a_3 then
@@ -117,19 +134,19 @@ let rec transitive_loop_z f s a_1 a_2 i =
    else
       true
 
-private type transitive_loop_yz_p 
-      (#a_t:Type) 
-      (f:cmp_t a_t) 
-      (s:seq a_t) 
-      (a_1:a_t) 
+private type transitive_loop_yz_p
+      (#a_t:Type)
+      (f:cmp_t a_t)
+      (s:seq a_t)
+      (a_1:a_t)
       (i:nat{i <= length s})
       =
    forall y z.
       (
-         mem_p y (slice s 0 i) 
-         /\ mem_p z s 
+         mem_p y (slice s 0 i)
+         /\ mem_p z s
          /\ b2t (f a_1 y && f y z)
-      ) 
+      )
       ==> f a_1 z
 
 private val transitive_loop_yz:
@@ -140,7 +157,7 @@ private val transitive_loop_yz:
    Tot (b:bool{b2t b <==> transitive_loop_yz_p f s a_1 (length s)})
       (decreases (length s - i))
 let rec transitive_loop_yz f s a_1 i =
-   slice_lemma s;
+   Flutterbye.Seq.Mem.slice_lemma s;
    if i < length s then
       let a_2 = index s i in
       if transitive_loop_z f s a_1 a_2 0 then
@@ -150,20 +167,19 @@ let rec transitive_loop_yz f s a_1 i =
    else
       true
 
-private type transitive_loop_xyz_p 
-      (#a_t:Type) 
-      (f:cmp_t a_t) 
-      (s:seq a_t) 
+private type transitive_loop_xyz_p
+      (#a_t:Type)
+      (f:cmp_t a_t)
+      (s:seq a_t)
       (i:nat{i <= length s})
       =
-   forall x y z.
-      (
-         mem_p x (slice s 0 i) 
-         /\ mem_p y s 
-         /\ mem_p z s 
-         /\ b2t (f x y && f y z)
-      ) 
-      ==> f x z
+   forall x y z. (
+      mem_p x (slice s 0 i)
+      /\ mem_p y s
+      /\ mem_p z s
+      /\ b2t (f x y && f y z)
+   )
+   ==> f x z
 
 private val transitive_loop_xyz:
    f:cmp_t 'a ->
@@ -172,7 +188,7 @@ private val transitive_loop_xyz:
    Tot (b:bool{b2t b <==> transitive_loop_xyz_p f s (length s)})
       (decreases (length s - i))
 let rec transitive_loop_xyz f s i =
-   slice_lemma s;
+   Flutterbye.Seq.Mem.slice_lemma s;
    if i < length s then
       let a_1 = index s i in
       if transitive_loop_yz f s a_1 0 then
@@ -189,8 +205,96 @@ private val transitive:
 let transitive f s =
    transitive_loop_xyz f s 0
 
+private type sequenced_loop_p (#a_t:Type) (f:cmp_t a_t) (s:seq a_t) (i:nat{i <= length s}) =
+   i < 2
+   \/ (forall (x:nat) (y:nat).
+         (x < i && y < i && x < y)
+         ==> (
+            x < i && y < i
+            && (
+               let a_x = index s x in
+               let a_y = index s y in
+               not (f a_y a_x) && (f a_x a_y)
+            )
+         )
+      )
+
+private val sequenced_loop:
+   f:cmp_t 'a ->
+   s:seq 'a{transitive_p f s} ->
+   i:nat{i <= length s /\ sequenced_loop_p f s i} ->
+   Tot (b:bool{b2t b <==> sequenced_loop_p f s (length s)})
+      (decreases (length s - i))
+let rec sequenced_loop f s i =
+   if i < length s then
+      begin
+         if i = 0 then
+            sequenced_loop f s 1
+         else
+            let a_0 = index s (i - 1) in
+            let a_i = index s i in
+            if not (f a_i a_0) && (f a_0 a_i) then
+               sequenced_loop f s (i + 1)
+            else
+               false
+      end
+   else
+      true
+
+private val sequenced:
+   f:cmp_t 'a ->
+   s:seq 'a{transitive_p f s} ->
+   Tot (b:bool{b2t b <==> sequenced_p f s})
+let rec sequenced f s =
+   sequenced_loop f s 0
+
 val pordered: f:cmp_t 'a -> s:seq 'a -> Tot (b:bool{b2t b <==> pordered_p f s})
 let pordered f s =
    reflexive_loop f s 0
    && antisymmetric_loop f s 0
    && transitive f s
+   && sequenced f s
+
+abstract val slice_lemma:
+   f:cmp_t 'a ->
+   s:seq 'a{pordered_p f s} ->
+   Lemma
+      (ensures
+         (forall (x:nat) (y:nat).
+            // if [x, y) describe a slice of `s`, then that slice is also partially ordered.
+            y <= length s && x <= y ==> pordered_p f (slice s x y)))
+let slice_lemma f s =
+   ()
+
+private val append_lemma_for_sequenced:
+   f:cmp_t 'a ->
+   s_1:seq 'a{sequenced_p f s_1} ->
+   s_2:seq 'a{sequenced_p f s_2} ->
+   Lemma
+      (ensures (sequenced_p f (append s_1 s_2)))
+let append_lemma_for_sequenced f s_1 s_2 =
+   if length s_1 = 0 || length s_2 = 0 then
+      ()
+   else
+      admit ()
+
+abstract val append_lemma:
+   f:cmp_t 'a ->
+   s_1:seq 'a{pordered_p f s_1} ->
+   s_2:seq 'a{pordered_p f s_2} ->
+   Lemma
+(*      (requires (
+         length s_1 > 0  && length s_2 > 0
+         ==> (
+            let a_1 = index s_1 (length s_1 - 1) in
+            let a_2 = index s_2 0 in
+            not (f a_2 a_1) && (f a_1 a_2)
+         )
+      ))*)
+      //(requires (sequenced_p f (append s_1 s_2))) // needed to prove.
+      (ensures (pordered_p f (append s_1 s_2)))
+let append_lemma f s_1 s_2 =
+   append_lemma_for_sequenced f s_1 s_2
+
+
+
